temp

backend/Cminor.v
@@ -234,7 +234,8 @@ Inductive state: Type :=
       forall (f: fundef)                (**r function to invoke *)
              (args: list val)           (**r arguments provided by caller *)
              (k: cont)                  (**r what to do next  *)
-             (m: mem),                  (**r memory state *)
+             (m: mem)                   (**r memory state *)
+             (id: ident),                (**r function id *)
       state
   | Returnstate:                (**r Return from a function *)
       forall (v: val)                   (**r Return value *)
@@ -438,11 +439,12 @@ Inductive step: state -> trace -> state -> Prop :=
   | step_skip_block: forall f k sp e m,
       step (State f Sskip (Kblock k) sp e m)
         E0 (State f Sskip k sp e m)
-  | step_skip_call: forall f k sp e m m',
+  | step_skip_call: forall f k sp e m m' m'',
       is_call_cont k ->
       Mem.free m sp 0 f.(fn_stackspace) = Some m' ->
+      Mem.return_frame m' = Some m'' ->
       step (State f Sskip k (Vptr sp Ptrofs.zero) e m)
-        E0 (Returnstate Vundef k m')
+        E0 (Returnstate Vundef k m'')
 
   | step_assign: forall f id a k sp e m v,
       eval_expr sp e m a v ->
@@ -456,22 +458,24 @@ Inductive step: state -> trace -> state -> Prop :=
       step (State f (Sstore chunk addr a) k sp e m)
         E0 (State f Sskip k sp e m')
 
-  | step_call: forall f optid sig a bl k sp e m vf vargs fd,
+  | step_call: forall f optid sig a bl k sp e m vf vargs fd id,
+      is_function_ident ge vf id ->
       eval_expr sp e m a vf ->
       eval_exprlist sp e m bl vargs ->
       Genv.find_funct ge vf = Some fd ->
       funsig fd = sig ->
       step (State f (Scall optid sig a bl) k sp e m)
-        E0 (Callstate fd vargs (Kcall optid f sp e k) m)
+        E0 (Callstate fd vargs (Kcall optid f sp e k) m id)
 
-  | step_tailcall: forall f sig a bl k sp e m vf vargs fd m',
+  | step_tailcall: forall f sig a bl k sp e m vf vargs fd m' id,
+      is_function_ident ge vf id ->
       eval_expr (Vptr sp Ptrofs.zero) e m a vf ->
       eval_exprlist (Vptr sp Ptrofs.zero) e m bl vargs ->
       Genv.find_funct ge vf = Some fd ->
       funsig fd = sig ->
       Mem.free m sp 0 f.(fn_stackspace) = Some m' ->
       step (State f (Stailcall sig a bl) k (Vptr sp Ptrofs.zero) e m)
-        E0 (Callstate fd vargs (call_cont k) m')
+        E0 (Callstate fd vargs (call_cont k) m' id)
 
   | step_builtin: forall f optid ef bl k sp e m vargs t vres m',
       eval_exprlist sp e m bl vargs ->
@@ -534,15 +538,14 @@ Inductive step: state -> trace -> state -> Prop :=
       step (State f (Sgoto lbl) k sp e m)
         E0 (State f s' k' sp e m)
 
-  | step_internal_function: forall f vargs k m m' m'' sp e,
-      Mem.alloc m 0 f.(fn_stackspace) = (m', sp) ->
-      Mem.alloc_frame m' = m'' ->
+  | step_internal_function: forall f vargs k m m' sp e id,
+      Mem.alloc (Mem.alloc_frame m id) 0 f.(fn_stackspace) = (m', sp) ->
       set_locals f.(fn_vars) (set_params vargs f.(fn_params)) = e ->
-      step (Callstate (Internal f) vargs k m)
-        E0 (State f f.(fn_body) k (Vptr sp Ptrofs.zero) e m'')
-  | step_external_function: forall ef vargs k m t vres m',
+      step (Callstate (Internal f) vargs k m id)
+        E0 (State f f.(fn_body) k (Vptr sp Ptrofs.zero) e m')
+  | step_external_function: forall ef vargs k m t vres m' id,
       external_call ef ge vargs m t vres m' ->
-      step (Callstate (External ef) vargs k m)
+      step (Callstate (External ef) vargs k m id)
          t (Returnstate vres k m')
 
   | step_return: forall v optid f sp e k m,
@@ -563,7 +566,7 @@ Inductive initial_state (p: program): state -> Prop :=
       Genv.find_symbol ge p.(prog_main) = Some b ->
       Genv.find_funct_ptr ge b = Some f ->
       funsig f = signature_main ->
-      initial_state p (Callstate f nil Kstop m0).
+      initial_state p (Callstate f nil Kstop m0 p.(prog_main)).
 
 (** A final state is a [Returnstate] with an empty continuation. *)
 
@@ -639,12 +642,17 @@ Proof.
   intros. constructor; set (ge := Genv.globalenv p); simpl; intros.
 - (* determ *)
   inv H; inv H0; Determ.
+  + assert (id = id0). eapply function_id_determ; eauto.
+    subst vf0 vargs0 id0. rewrite H4 in H18. inv H18. auto.
+  + assert (id = id0). eapply function_id_determ; eauto.
+    subst vf0 vargs0 id0. rewrite H4 in H18. inv H18.
+    rewrite H6 in H20. inv H20. auto.
   + subst vargs0. exploit external_call_determ. eexact H2. eexact H13.
     intros (A & B). split; intros; auto.
     apply B in H; destruct H; congruence.
   + subst v0. assert (b0 = b) by (inv H2; inv H13; auto). subst b0; auto.
   + assert (n0 = n) by (inv H2; inv H14; auto). subst n0; auto.
-  + exploit external_call_determ. eexact H1. eexact H7.
+  + exploit external_call_determ. eexact H1. eexact H8.
     intros (A & B). split; intros; auto.
     apply B in H; destruct H; congruence.
 - (* single event *)
