backend/RTL.v
@@ -171,7 +171,8 @@ Inductive state : Type :=
       forall (stack: list stackframe) (**r call stack *)
              (f: fundef)              (**r function to call *)
              (args: list val)         (**r arguments to the call *)
-             (m: mem),                (**r memory state *)
+             (m: mem)                 (**r memory state *)
+             (id: ident),             (**r function ident *)
       state
   | Returnstate:
       forall (stack: list stackframe) (**r call stack *)
@@ -198,6 +199,11 @@ Definition find_function
   [step ge st1 t st2], where [ge] is the global environment,
   [st1] the initial state, [st2] the final state, and [t] the trace
   of system calls performed during this transition. *)
+Definition ros_is_function (ros: reg + ident) (rs: regset) (i: ident) : Prop :=
+  match ros with
+  | inl r => exists b o, rs # r = Vptr b o /\ Genv.find_symbol ge i = Some b
+  | inr symb => i = symb
+  end.
 
 Inductive step: state -> trace -> state -> Prop :=
   | exec_Inop:
@@ -226,21 +232,23 @@ Inductive step: state -> trace -> state -> Prop :=
       step (State s f sp pc rs m)
         E0 (State s f sp pc' rs m')
   | exec_Icall:
-      forall s f sp pc rs m sig ros args res pc' fd,
+      forall s f sp pc rs m sig ros args res pc' fd id,
+      ros_is_function ros rs id ->
       (fn_code f)!pc = Some(Icall sig ros args res pc') ->
       find_function ros rs = Some fd ->
       funsig fd = sig ->
       step (State s f sp pc rs m)
-        E0 (Callstate (Stackframe res f sp pc' rs :: s) fd rs##args m)
+        E0 (Callstate (Stackframe res f sp pc' rs :: s) fd rs##args m id)
   | exec_Itailcall:
-      forall s f stk pc rs m sig ros args fd m' m'', 
+      forall s f stk pc rs m sig ros args fd m' m'' id,
+      ros_is_function ros rs id ->
       (fn_code f)!pc = Some(Itailcall sig ros args) ->
       find_function ros rs = Some fd ->
       funsig fd = sig ->
       Mem.free m stk 0 f.(fn_stacksize) = Some m' ->
       Mem.return_frame m' = Some m'' ->
       step (State s f (Vptr stk Ptrofs.zero) pc rs m)
-        E0 (Callstate s fd rs##args m'')
+        E0 (Callstate s fd rs##args m'' id)
   | exec_Ibuiltin:
       forall s f sp pc rs m ef args res pc' vargs t vres m',
       (fn_code f)!pc = Some(Ibuiltin ef args res pc') ->
@@ -270,9 +278,9 @@ Inductive step: state -> trace -> state -> Prop :=
       step (State s f (Vptr stk Ptrofs.zero) pc rs m)
         E0 (Returnstate s (regmap_optget or Vundef rs) m'')
   | exec_function_internal:
-      forall s f args m m' stk,
-      Mem.alloc (Mem.alloc_frame m) 0 f.(fn_stacksize) = (m', stk) ->
-      step (Callstate s (Internal f) args m)
+      forall s f args m m' stk id,
+      Mem.alloc (Mem.alloc_frame m id) 0 f.(fn_stacksize) = (m', stk) ->
+      step (Callstate s (Internal f) args m id)
         E0 (State s
                   f
                   (Vptr stk Ptrofs.zero)
@@ -280,9 +288,9 @@ Inductive step: state -> trace -> state -> Prop :=
                   (init_regs args f.(fn_params))
                   m')
   | exec_function_external:
-      forall s ef args res t m m',
-      external_call ef ge args m t res m' ->
-      step (Callstate s (External ef) args m)
+      forall s ef args res t m m' id,
+      external_call ef ge args m t res m'->
+      step (Callstate s (External ef) args m id)
          t (Returnstate s res m')
   | exec_return:
       forall res f sp pc rs s vres m,
@@ -326,7 +334,7 @@ Inductive initial_state (p: program): state -> Prop :=
       Genv.find_symbol ge p.(prog_main) = Some b ->
       Genv.find_funct_ptr ge b = Some f ->
       funsig f = signature_main ->
-      initial_state p (Callstate nil f nil m0).
+      initial_state p (Callstate nil f nil m0 p.(prog_main)).
 
 (** A final state is a [Returnstate] with an empty call stack. *)
 
