cfrontend/Cminorgenproof.v
@@ -1613,6 +1613,7 @@ Inductive match_states: Csharpminor.state -> Cminor.state -> Prop :=
       (TRF: transl_funbody cenv sz fn = OK tfn)
       (TR: transl_stmt cenv xenv s = OK ts)
       (MINJ: Mem.inject f m tm)
+      (STACK: Mem.stack_feq m tm)
       (MCS: match_callstack f m tm
                (Frame cenv tfn e le te sp sps bes es :: cs)
                (Mem.support m) (Mem.support tm))
@@ -1625,6 +1626,7 @@ Inductive match_states: Csharpminor.state -> Cminor.state -> Prop :=
       (TRF: transl_funbody cenv sz fn = OK tfn)
       (TR: transl_stmt cenv xenv s1 = OK ts1)
       (MINJ: Mem.inject f m tm)
+      (STACK: Mem.stack_feq m tm)
       (MCS: match_callstack f m tm
                (Frame cenv tfn e le te sp sps bes es :: cs)
                (Mem.support m) (Mem.support tm))
@@ -1632,18 +1634,20 @@ Inductive match_states: Csharpminor.state -> Cminor.state -> Prop :=
       match_states (Csharpminor.State fn (Csharpminor.Sseq s1 s2) k e le m)
                    (State tfn ts1 tk (Vptr sp Ptrofs.zero) te tm)
   | match_callstate:
-      forall fd args k m tfd targs tk tm f cs cenv
+      forall fd args k m tfd targs tk tm f cs cenv id
       (TR: transl_fundef fd = OK tfd)
       (MINJ: Mem.inject f m tm)
+      (STACK: Mem.stack_feq m tm)
       (MCS: match_callstack f m tm cs (Mem.support m) (Mem.support tm))
       (MK: match_cont k tk cenv nil cs)
       (ISCC: Csharpminor.is_call_cont k)
       (ARGSINJ: Val.inject_list f args targs),
-      match_states (Csharpminor.Callstate fd args k m)
-                   (Callstate tfd targs tk tm)
+      match_states (Csharpminor.Callstate fd args k m id)
+                   (Callstate tfd targs tk tm id)
   | match_returnstate:
       forall v k m tv tk tm f cs cenv
       (MINJ: Mem.inject f m tm)
+      (STACK: Mem.stack_feq m tm)
       (MCS: match_callstack f m tm cs (Mem.support m) (Mem.support tm))
       (MK: match_cont k tk cenv nil cs)
       (RESINJ: Val.inject f v tv),
@@ -1819,6 +1823,7 @@ Lemma switch_match_states:
     (TRF: transl_funbody cenv sz fn = OK tfn)
     (TR: transl_lblstmt cenv (switch_env ls xenv) ls body = OK ts)
     (MINJ: Mem.inject f m tm)
+    (STACK: Mem.stack_feq m tm)
     (MCS: match_callstack f m tm
                (Frame cenv tfn e le te sp sps bes es :: cs)
                (Mem.support m) (Mem.support tm))
@@ -2002,9 +2007,12 @@ Proof.
   monadInv TR. left.
   exploit match_is_call_cont; eauto. intros [tk' [A [B C]]].
   exploit match_callstack_freelist; eauto. intros [tm' [P [Q R]]].
+  exploit Mem.return_frame_parallel_inject; eauto.
   econstructor; split.
-  eapply plus_right. eexact A. apply step_skip_call. auto. eauto. traceEq.
-  econstructor; eauto.
+  eapply plus_right. eexact A. eapply step_skip_call. eauto. eauto.
+  admit.
+  traceEq.
+  econstructor; eauto. admit. admit.
 
 (* set *)
   monadInv TR.
@@ -2043,6 +2051,8 @@ Proof.
   intros [tvargs [EVAL2 VINJ2]].
   left; econstructor; split.
   apply plus_one. eapply step_call; eauto.
+  destruct H as (bb & oo & EQ3 & EQ2). red; rewrite EQ3.
+  rewrite symbols_preserved; eauto.
   apply sig_preserved; eauto.
   econstructor; eauto.
   eapply match_Kcall with (cenv' := cenv); eauto.
@@ -2060,7 +2070,7 @@ Proof.
   apply plus_one. econstructor. eauto.
   eapply external_call_symbols_preserved; eauto. apply senv_preserved.
   assert (MCS': match_callstack f' m' tm'
-                 (Frame cenv tfn e le te (fresh_block true sps) sps bes es :: cs)
+                 (Frame cenv tfn e le te (fresh_block sps) sps bes es :: cs)
                  (Mem.support m') (Mem.support tm')).
     apply match_callstack_incr_bound with (Mem.support m) (Mem.support tm).
     eapply match_callstack_external_call; eauto.
@@ -2087,7 +2097,7 @@ Opaque PTree.set.
 (* ifthenelse *)
   monadInv TR.
   exploit transl_expr_correct; eauto. intros [tv [EVAL VINJ]].
-  left; exists (State tfn (if b then x0 else x1) tk (Vptr (fresh_block true sps) Ptrofs.zero) te tm); split.
+  left; exists (State tfn (if b then x0 else x1) tk (Vptr (fresh_block sps) Ptrofs.zero) te tm); split.
   apply plus_one. eapply step_ifthenelse; eauto. eapply bool_of_val_inject; eauto.
   econstructor; eauto. destruct b; auto.
 
@@ -2160,8 +2170,8 @@ Opaque PTree.set.
   monadInv TR. left.
   exploit match_callstack_freelist; eauto. intros [tm' [A [B C]]].
   econstructor; split.
-  apply plus_one. eapply step_return_0. eauto.
-  econstructor; eauto. eapply match_call_cont; eauto.
+  apply plus_one. eapply step_return_0. eauto. admit.
+  econstructor; eauto. admit. admit. eapply match_call_cont; eauto.
   simpl; auto.
 
 (* return some *)
@@ -2169,7 +2179,7 @@ Opaque PTree.set.
   exploit transl_expr_correct; eauto. intros [tv [EVAL VINJ]].
   exploit match_callstack_freelist; eauto. intros [tm' [A [B C]]].
   econstructor; split.
-  apply plus_one. eapply step_return_1. eauto. eauto.
+  apply plus_one. eapply step_return_1. eauto. eauto. admit.
   econstructor; eauto. eapply match_call_cont; eauto.
 
 (* label *)
@@ -2197,14 +2207,16 @@ Opaque PTree.set.
                         (Csharpminor.fn_temps f)
                         sz
                         x0) in *.
-  caseEq (Mem.alloc true tm 0 (fn_stackspace tf)). intros tm' sp ALLOC'.
+  caseEq (Mem.alloc (Mem.alloc_frame tm id) 0 (fn_stackspace tf)). intros tm' sp ALLOC'.
   exploit match_callstack_function_entry; eauto. simpl; eauto. simpl; auto.
+  admit. eapply Mem.alloc_frame_parallel_inject. auto.
   intros [f2 [MCS2 MINJ2]].
   left; econstructor; split.
   apply plus_one. constructor; simpl; eauto.
   econstructor. eapply Mem.alloc_result. eauto.
   eexact TRBODY. eauto. eexact MINJ2. eexact MCS2.
-  inv MK; simpl in ISCC; contradiction || econstructor; eauto.
+  inv MK; simpl in ISCC. econstructor. contradiction.
+  econstructor. contradiction. contradiction. econstructor; eauto.
 
 (* external call *)
   monadInv TR.
@@ -2230,7 +2242,7 @@ Opaque PTree.set.
   apply plus_one. econstructor; eauto.
   unfold set_optvar. destruct optid; simpl; econstructor; eauto.
   eapply match_callstack_set_temp; eauto.
-Qed.
+Admitted.
 
 Lemma match_globalenvs_init:
   forall m,
@@ -2261,6 +2273,7 @@ Proof.
   eapply match_program_main; eauto.
   eexact FIND.
   rewrite <- H2. apply sig_preserved; auto.
+  destruct TRANSL as (_&MAIN&_). rewrite MAIN.
   eapply match_callstate with (f := Mem.flat_inj (Mem.support m0)) (cs := @nil frame) (cenv := PTree.empty Z).
   auto.
   eapply Genv.initmem_inject; eauto.
